Some minor progress and started the Coq <-> Lean tactics cheat-sheet

SoftwareFoundations/LogicalFoundations/ImpCEvalFun.lean
@@ -4,3 +4,91 @@
 
 import «SoftwareFoundations».«LogicalFoundations».«Maps»
 import «SoftwareFoundations».«LogicalFoundations».«Imp»
+
+import Mathlib.Tactic.Relation.Trans
+
+/-
+## A Broken Evaluator
+-/
+
+def Command.broken (state: State): Command → State
+  | .skip => state
+  | .assign id e => state.update id (e.eval state)
+  | .seq c₁ c₂ =>
+    state
+      |> c₁.broken
+      |> c₂.broken
+  | .if c t f =>
+    if c.eval state
+    then t.broken state
+    else f.broken state
+  | .while _ _ => state
+
+/-
+## A Step-Indexed Evaluator
+-/
+
+def Command.eval (state: State): Nat → Command → Option State
+  | 0, _ => .none
+  | .succ _, .skip => .some state
+  | .succ _, .assign id e => .some (state.update id (e.eval state))
+  | .succ i, .seq c₁ c₂ =>
+    let state := c₁.eval state i
+    match state with
+      | .none => .none
+      | .some state => c₂.eval state i
+  | .succ i, .if c t f =>
+    if c.eval state
+    then t.eval state i
+    else f.eval state i
+  | .succ i, .while c b =>
+    if c.eval state
+    then
+      match b.eval state i with
+        | .none => .none
+        | .some state => (Command.while c b).eval state i
+    else .some state
+
+def Command.eval_test (state: State) (c: Command): Option (Nat × Nat × Nat) :=
+  match c.eval state 100 with
+    | .none => .none
+    | .some state => .some (state "X", state "Y", state "Z")
+
+example: (Command.seq (.assign "X" 2) (.if (.le "X" 1) (.assign "Y" 3) (.assign "Z" 4))).eval_test State.empty = .some (2, 0, 4) := rfl
+
+-- TODO: Pup
+
+def pEven: Command :=
+  (.while (.gt "X" 1)
+    (.assign "X" (.minus "X" 2)))
+
+example: pEven.eval_test (State.build [("X", 0)]) = .some (0, 0, 0) := rfl
+example: pEven.eval_test (State.build [("X", 1)]) = .some (1, 0, 0) := rfl
+example: pEven.eval_test (State.build [("X", 2)]) = .some (0, 0, 0) := rfl
+example: pEven.eval_test (State.build [("X", 3)]) = .some (1, 0, 0) := rfl
+example: pEven.eval_test (State.build [("X", 42)]) = .some (0, 0, 0) := rfl
+example: pEven.eval_test (State.build [("X", 43)]) = .some (1, 0, 0) := rfl
+example: pEven.eval_test (State.build [("X", 200)]) = .none := rfl
+
+/-
+## Relational vs. Step-Indexed Evaluation
+-/
+
+theorem Command.eval.equiv_rel (c: Command) (s₁ s₂: State): (∃ i: Nat, c.eval s₁ i = .some s₂) → CommandEval c s₁ s₂ := by
+  sorry
+
+theorem Command.eval.step (c: Command) (s₁ s₂: State) (h: CommandEval c s₁ s₂): ∃ i: Nat, c.eval s₁ i = .some s₂ := by
+  sorry
+  where
+    more (i₁ i₂: Nat) (s₁ s₂: State) (c: Command) (h₁: i₁ ≤ i₂) (h₂: c.eval s₁ i₁ = s₂): c.eval s₁ i₂ = s₂ := by
+      sorry
+
+theorem Command.eval.equiv_step (c: Command) (s₁ s₂: State): CommandEval c s₁ s₂ ↔ ∃ i: Nat, c.eval s₁ i = .some s₂ := by
+  sorry
+
+/-
+## Determinism of Evaluation Again
+-/
+
+theorem CommandEval.deterministic.better (c: Command) (s₁ s₂ s₃: State) (h₁: CommandEval c s₁ s₂) (h₂: CommandEval c s₁ s₃): s₂ = s₃ := by
+  sorry
