SoftwareFoundations/LogicalFoundations/Extraction.lean
@@ -1,3 +1,6 @@
 /-
 # Extracting OCaml from Coq
 -/
+
+-- Lean is itself a useful functional programming language that compiles to
+-- native code, so there no need to extract anything.  :)
